Share effects definition across CBPV/CBV

coq/CBV/cbv.sig
@@ -1,17 +1,6 @@
-type : Type
 bool : Type
-effect : Type
 Value : Type
 Exp : Type
-
-Tick : effect
-Add : effect -> effect -> effect
-Pure : effect
-
-Unit : type 
-Arr : type -> effect -> type -> type 
-Cross : type -> type -> type 
-Plus : type -> type -> type 
 
 One : Value
 Lam : (Value -> Exp) -> Value 
