coq/CBV/CBV.v
@@ -2,44 +2,6 @@ Require Export fintype.
 
 
 
-Section effect.
-Inductive effect  : Type :=
-  | Tick : effect 
-  | Add : effect   -> effect   -> effect 
-  | Pure : effect .
-
-Lemma congr_Tick  : Tick  = Tick  .
-Proof. congruence. Qed.
-
-Lemma congr_Add  { s0 : effect   } { s1 : effect   } { t0 : effect   } { t1 : effect   } (H1 : s0 = t0) (H2 : s1 = t1) : Add s0 s1 = Add t0 t1 .
-Proof. congruence. Qed.
-
-Lemma congr_Pure  : Pure  = Pure  .
-Proof. congruence. Qed.
-
-End effect.
-
-Section type.
-Inductive type  : Type :=
-  | Unit : type 
-  | Arr : type   -> effect   -> type   -> type 
-  | Cross : type   -> type   -> type 
-  | Plus : type   -> type   -> type .
-
-Lemma congr_Unit  : Unit  = Unit  .
-Proof. congruence. Qed.
-
-Lemma congr_Arr  { s0 : type   } { s1 : effect   } { s2 : type   } { t0 : type   } { t1 : effect   } { t2 : type   } (H1 : s0 = t0) (H2 : s1 = t1) (H3 : s2 = t2) : Arr s0 s1 s2 = Arr t0 t1 t2 .
-Proof. congruence. Qed.
-
-Lemma congr_Cross  { s0 : type   } { s1 : type   } { t0 : type   } { t1 : type   } (H1 : s0 = t0) (H2 : s1 = t1) : Cross s0 s1 = Cross t0 t1 .
-Proof. congruence. Qed.
-
-Lemma congr_Plus  { s0 : type   } { s1 : type   } { t0 : type   } { t1 : type   } (H1 : s0 = t0) (H2 : s1 = t1) : Plus s0 s1 = Plus t0 t1 .
-Proof. congruence. Qed.
-
-End type.
-
 
 Section ValueExp.
 Inductive Value (nValue : nat) : Type :=
